FStar.UInt: tame a hard proof
Goes through way quicker

ulib/FStar.UInt.fst
@@ -823,12 +823,16 @@ val lemma_msb_pow2: #n:pos -> a:uint_t n ->
   Lemma (msb a <==> a >= pow2 (n-1))
 let lemma_msb_pow2 #n a = if n = 1 then () else from_vec_propriety (to_vec a) 1
 
-#set-options "--z3rlimit 80 --initial_fuel 1 --max_fuel 1 --max_ifuel 0"
+private val plus_one_mod : p:pos -> a:nat ->
+    Lemma (requires (a < p /\ ((a + 1) % p == 0))) (ensures (a == p - 1))
+private let plus_one_mod p a = ()
+
 val lemma_minus_zero: #n:pos -> a:uint_t n ->
   Lemma (minus a = 0 ==> a = 0)
 let lemma_minus_zero #n a =
   if minus a = 0 then
   begin
+    plus_one_mod (pow2 n) (lognot a);
     lognot_self a;
     logxor_self (ones n);
     logxor_lemma_2 #n (ones n)
